src/dafny/beacon/statetransition/ProcessOperations.p.dfy
@@ -16,13 +16,16 @@ include "../../utils/NativeTypes.dfy"
 include "../../utils/Eth2Types.dfy"
 include "../../utils/Helpers.dfy"
 include "../../utils/MathHelpers.dfy"
+include "../../utils/SeqHelpers.dfy"
 include "../../ssz/Constants.dfy"
 include "../BeaconChainTypes.dfy"
 include "../validators/Validators.dfy"
+include "../validators/ValidatorHelpers.dfy"
 include "../attestations/AttestationsTypes.dfy"
 include "../attestations/AttestationsHelpers.dfy"
 include "../Helpers.dfy"
-include "ProcessOperations.dfy"
+include "../Helpers.s.dfy"
+//include "ProcessOperations.dfy"
 
 /**
  *  Proofs for process operations
@@ -35,11 +38,14 @@ module ProcessOperationsProofs {
     import opened Constants
     import opened BeaconChainTypes
     import opened Validators
+    import opened ValidatorHelpers
     import opened AttestationsTypes
     import opened AttestationsHelpers
     import opened BeaconHelpers
+    import opened BeaconHelperSpec
     import opened MathHelpers
-    import ProcessOperations
+    import opened SeqHelpers
+    //import ProcessOperations
 
     
     // Helper lemmas
@@ -96,7 +102,107 @@ module ProcessOperationsProofs {
 
 
 
+// lemma updateBalTotalBySingleDeposit(s: BeaconState, d: Deposit)
+//         requires s.eth1_deposit_index as int +  1 < 0x10000000000000000 
+//         requires |s.validators| == |s.balances|
+//         requires |s.validators| + 1 <= VALIDATOR_REGISTRY_LIMIT as int
+//         requires total_balances(s.balances) + d.data.amount as int < 0x10000000000000000
+        
+//         ensures total_balances(updateDeposit(s,d).balances) == total_balances(s.balances) + d.data.amount as int < 0x10000000000000000
+//         //ensures total_balances(updateDeposit(s,d).balances) == total_balances(s.balances) + total_deposits([d]) 
+//     {
+//         var pk := seqKeysInValidators(s.validators); 
+//         if |s.balances| == 0 {
+//             // Thanks Dafny
+//         }
+//         else {
+//             if d.data.pubkey in pk {
+//                 var index := get_validator_index(pk, d.data.pubkey);
+//                 individualBalanceBoundMaintained(s.balances,d);
+//                 //assert updateDeposit(s,d).balances ==  increase_balance(s,index,d.data.amount).balances;
+//                 //assert increase_balance(s,index,d.data.amount).balances[index] == s.balances[index] + d.data.amount;
+//                 //assert forall i :: 0 <= i < |s.balances| && i != index as int ==> increase_balance(s,index,d.data.amount).balances[i] == s.balances[i];
+//                 //assert total_balances(updateDeposit(s,d).balances) == total_balances(increase_balance(s,index,d.data.amount).balances) ;
+//                 updateExistingBalance(s, index, d.data.amount);
+//                 //assert total_balances(updateDeposit(s,d).balances) == total_balances(s.balances) + d.data.amount as int ;
+//             }
+//             else {
+//                 //assert updateDeposit(s,d).balances == s.balances + [d.data.amount];
+//                 distBalancesProp(s.balances,[d.data.amount]);
+//                 //assert total_balances(s.balances + [d.data.amount]) == total_balances(s.balances) + total_balances([d.data.amount]);
+//             }
+//         }
+//     }
+
+
 ///////////////////////////
+    lemma testLemma3(s: BeaconState, s2: BeaconState, ps1: seq<ProposerSlashing>, ps2: ProposerSlashing, ps: seq<ProposerSlashing>)
+        requires |ps1| == |ps|-1
+        requires ps1 == ps[..|ps|-1]
+        requires ps2 == ps[|ps|-1]
+
+        requires forall i,j :: 0 <= i < j < |ps| && i != j ==> ps[i].header_1.proposer_index!= ps[j].header_1.proposer_index 
+        requires forall i :: 0 <= i < |ps1| ==> ps1[i].header_1.proposer_index as int < |s.validators| 
+        requires ps2.header_1.proposer_index as int < |s.validators| 
+        requires |s2.validators| == |s.validators|
+
+        requires forall i :: 0 <= i < |s.validators| && i !in (get_PS_validator_indices(ps1) + [ps2.header_1.proposer_index as int]) 
+                ==> s2.validators[i] == s.validators[i]
+        
+        ensures forall i :: 0 <= i < |s.validators| && i !in get_PS_validator_indices(ps) ==> s2.validators[i] == s.validators[i]
+    {
+        seqInitLast<ProposerSlashing>(ps, |ps|-1);
+        assert ps[..|ps|-1] + [ps[|ps|-1]] == ps[..|ps|];
+        assert ps[..|ps|] == ps;
+        assert ps1 + [ps2] == ps; 
+
+        subsetMappingPSIndices(ps,|ps|-1);
+        assert ps1 == ps[..|ps|-1];
+        assert get_PS_validator_indices(ps[..|ps|-1]) == get_PS_validator_indices(ps1) == get_PS_validator_indices(ps)[..|ps|-1];
+
+        ////////
+        mappingPSIndices(ps);
+        assert forall i :: 0 <= i < |ps| ==> get_PS_validator_indices(ps)[i] == ps[i].header_1.proposer_index as int;
+        assert get_PS_validator_indices(ps)[|ps|-1] == ps[|ps|-1].header_1.proposer_index as int == ps2.header_1.proposer_index as int;
+
+        assert get_PS_validator_indices(ps)[..|ps|-1] + [get_PS_validator_indices(ps)[|ps|-1]] == get_PS_validator_indices(ps);
+    
+        assert get_PS_validator_indices(ps1) + [ps2.header_1.proposer_index as int] == get_PS_validator_indices(ps);
+
+    }
+
+
+
+
+    lemma testLemma1(s: BeaconState, s1: BeaconState, ps1: seq<ProposerSlashing>, ps2: ProposerSlashing, ps: seq<ProposerSlashing>)
+        requires |ps1| == |ps|-1
+        requires ps1 == ps[..|ps|-1]
+        requires ps2 == ps[|ps|-1]
+
+        //requires ps1 + [ps2] == ps
+        requires forall i,j :: 0 <= i < j < |ps| && i != j ==> ps[i].header_1.proposer_index!= ps[j].header_1.proposer_index 
+        requires forall i :: 0 <= i < |ps1| ==> ps1[i].header_1.proposer_index as int < |s.validators| 
+        requires ps2.header_1.proposer_index as int < |s.validators| 
+        requires |s1.validators| == |s.validators|
+
+        requires forall i :: 0 <= i < |s.validators| && i !in get_PS_validator_indices(ps1) ==> s1.validators[i] == s.validators[i]
+        requires ps2 !in ps1
+
+        ensures s1.validators[ps2.header_1.proposer_index] == s.validators[ps2.header_1.proposer_index]
+    {
+        seqInitLast<ProposerSlashing>(ps, |ps|-1);
+        assert ps[..|ps|-1] + [ps[|ps|-1]] == ps[..|ps|];
+        assert ps[..|ps|] == ps;
+        assert ps1 + [ps2] == ps;
+        
+        mappingPSIndices(ps1);
+        assert forall i :: 0 <= i < |ps1| ==> get_PS_validator_indices(ps1)[i] == ps1[i].header_1.proposer_index as int;
+        assert forall i :: 0 <= i < |ps[..|ps|-1]|  ==> ps[i].header_1.proposer_index != ps[|ps|-1].header_1.proposer_index ;
+        assert ps2.header_1.proposer_index as int !in get_PS_validator_indices(ps1);
+    }
+
+
+
     lemma mappingPSIndices(ps: seq<ProposerSlashing>)
         ensures forall i :: 0 <= i < |ps| ==> get_PS_validator_indices(ps)[i] == ps[i].header_1.proposer_index as int
     {
@@ -119,167 +225,159 @@ module ProcessOperationsProofs {
         }
     }
 
-    lemma helperPSLemma(s: BeaconState, ps: ProposerSlashing)
-        requires ps.header_1.slot == ps.header_2.slot
-        requires ps.header_1.proposer_index == ps.header_2.proposer_index 
-        requires ps.header_1 == ps.header_2
-        requires ps.header_1.proposer_index as int < |s.validators| 
+    // lemma helperPSLemma(s: BeaconState, ps: ProposerSlashing)
+    //     requires ps.header_1.slot == ps.header_2.slot
+    //     requires ps.header_1.proposer_index == ps.header_2.proposer_index 
+    //     requires ps.header_1 == ps.header_2
+    //     requires ps.header_1.proposer_index as int < |s.validators| 
 
-        // requires is_active_validator: (!v.slashed) && (v.activation_epoch <= epoch < v.withdrawable_epoch)
-        requires !s.validators[ps.header_1.proposer_index].slashed
-        requires s.validators[ps.header_1.proposer_index].activation_epoch <= get_current_epoch(s) < s.validators[ps.header_1.proposer_index].withdrawable_epoch
+    //     // requires is_active_validator: (!v.slashed) && (v.activation_epoch <= epoch < v.withdrawable_epoch)
+    //     requires !s.validators[ps.header_1.proposer_index].slashed
+    //     requires s.validators[ps.header_1.proposer_index].activation_epoch <= get_current_epoch(s) < s.validators[ps.header_1.proposer_index].withdrawable_epoch
  
-        requires |get_active_validator_indices(s.validators, get_current_epoch(s))| > 0
-        requires |s.validators| == |s.balances|
+    //     requires |get_active_validator_indices(s.validators, get_current_epoch(s))| > 0
+    //     requires |s.validators| == |s.balances|
         
-        ensures forall i :: 0 <= i < |s.validators| && i != ps.header_1.proposer_index as int ==> updateProposerSlashing(s, ps).validators[i].exitEpoch == s.validators[i].exitEpoch
-        ensures forall i :: 0 <= i < |s.validators| && i != ps.header_1.proposer_index as int ==> updateProposerSlashing(s, ps).validators[i].slashed == s.validators[i].slashed
-        ensures forall i :: 0 <= i < |s.validators| && i != ps.header_1.proposer_index as int ==> updateProposerSlashing(s, ps).validators[i].withdrawable_epoch == s.validators[i].withdrawable_epoch
-    {
-        // Thanks Dafny
-    }
+    //     ensures forall i :: 0 <= i < |s.validators| && i != ps.header_1.proposer_index as int ==> updateProposerSlashing(s, ps).validators[i].exitEpoch == s.validators[i].exitEpoch
+    //     ensures forall i :: 0 <= i < |s.validators| && i != ps.header_1.proposer_index as int ==> updateProposerSlashing(s, ps).validators[i].slashed == s.validators[i].slashed
+    //     ensures forall i :: 0 <= i < |s.validators| && i != ps.header_1.proposer_index as int ==> updateProposerSlashing(s, ps).validators[i].withdrawable_epoch == s.validators[i].withdrawable_epoch
+    // {
+    //     // Thanks Dafny
+    //}
 
-    lemma helperPSLemma2(s: BeaconState, ps: seq<ProposerSlashing>)
-        requires  |get_PS_validator_indices(ps)| > 0
-        requires forall i :: i in get_PS_validator_indices(ps) ==> 0 <= i < |s.validators| 
-        requires forall i :: i in get_PS_validator_indices(ps) ==> !s.validators[i].slashed
-        requires forall i :: i in get_PS_validator_indices(ps) ==> s.validators[i].activation_epoch <= get_current_epoch(s) < s.validators[i].withdrawable_epoch
+    // lemma helperPSLemma2(s: BeaconState, ps: seq<ProposerSlashing>)
+    //     requires  |get_PS_validator_indices(ps)| > 0
+    //     requires forall i :: i in get_PS_validator_indices(ps) ==> 0 <= i < |s.validators| 
+    //     requires forall i :: i in get_PS_validator_indices(ps) ==> !s.validators[i].slashed
+    //     requires forall i :: i in get_PS_validator_indices(ps) ==> s.validators[i].activation_epoch <= get_current_epoch(s) < s.validators[i].withdrawable_epoch
         
 
-        ensures forall i :: i in get_PS_validator_indices(ps[..|ps|-1]) ==> 0 <= i < |s.validators|
-        ensures forall i :: i in get_PS_validator_indices(ps[..|ps|-1]) ==> !s.validators[i].slashed
-        ensures forall i :: i in get_PS_validator_indices(ps[..|ps|-1]) ==> s.validators[i].activation_epoch <= get_current_epoch(s) < s.validators[i].withdrawable_epoch
-    {
-        mappingPSIndices(ps);
-        assert forall i :: 0 <= i < |ps| ==> get_PS_validator_indices(ps)[i] == ps[i].header_1.proposer_index as int;
+    //     ensures forall i :: i in get_PS_validator_indices(ps[..|ps|-1]) ==> 0 <= i < |s.validators|
+    //     ensures forall i :: i in get_PS_validator_indices(ps[..|ps|-1]) ==> !s.validators[i].slashed
+    //     ensures forall i :: i in get_PS_validator_indices(ps[..|ps|-1]) ==> s.validators[i].activation_epoch <= get_current_epoch(s) < s.validators[i].withdrawable_epoch
+    // {
+    //     mappingPSIndices(ps);
+    //     assert forall i :: 0 <= i < |ps| ==> get_PS_validator_indices(ps)[i] == ps[i].header_1.proposer_index as int;
 
-        subsetMappingPSIndices(ps, |ps|-1);
-        assert get_PS_validator_indices(ps[..|ps|-1]) == get_PS_validator_indices(ps)[..|ps|-1];
+    //     subsetMappingPSIndices(ps, |ps|-1);
+    //     assert get_PS_validator_indices(ps[..|ps|-1]) == get_PS_validator_indices(ps)[..|ps|-1];
         
-        assert forall i :: i in get_PS_validator_indices(ps) ==> 0 <= i < |s.validators|; // from requires
-        assert forall i :: 0 <= i < |ps| ==> get_PS_validator_indices(ps)[i] == ps[i].header_1.proposer_index as int;
-        assert forall i :: 0 <= i < |ps| ==> ps[i].header_1.proposer_index as int in get_PS_validator_indices(ps) ;
+    //     assert forall i :: i in get_PS_validator_indices(ps) ==> 0 <= i < |s.validators|; // from requires
+    //     assert forall i :: 0 <= i < |ps| ==> get_PS_validator_indices(ps)[i] == ps[i].header_1.proposer_index as int;
+    //     assert forall i :: 0 <= i < |ps| ==> ps[i].header_1.proposer_index as int in get_PS_validator_indices(ps) ;
         
-    }
+    // }
 
 
-    lemma updateProposerSlashingLemma(s: BeaconState, ps : ProposerSlashing)
-        requires ps.header_1.slot == ps.header_2.slot
-        requires ps.header_1.proposer_index == ps.header_2.proposer_index 
-        requires ps.header_1 == ps.header_2
-        requires ps.header_1.proposer_index as int < |s.validators| 
-        //requires is_slashable_validator(s.validators[ps.header_1.proposer_index], get_current_epoch(s));
-        //(!v.slashed) && (v.activation_epoch <= epoch < v.withdrawable_epoch)
-        requires !s.validators[ps.header_1.proposer_index].slashed
-        requires s.validators[ps.header_1.proposer_index].activation_epoch <= get_current_epoch(s) < s.validators[ps.header_1.proposer_index].withdrawable_epoch
+    // lemma updateProposerSlashingLemma(s: BeaconState, ps : ProposerSlashing)
+    //     requires ps.header_1.slot == ps.header_2.slot
+    //     requires ps.header_1.proposer_index == ps.header_2.proposer_index 
+    //     requires ps.header_1 == ps.header_2
+    //     requires ps.header_1.proposer_index as int < |s.validators| 
+    //     //requires is_slashable_validator(s.validators[ps.header_1.proposer_index], get_current_epoch(s));
+    //     //(!v.slashed) && (v.activation_epoch <= epoch < v.withdrawable_epoch)
+    //     requires !s.validators[ps.header_1.proposer_index].slashed
+    //     requires s.validators[ps.header_1.proposer_index].activation_epoch <= get_current_epoch(s) < s.validators[ps.header_1.proposer_index].withdrawable_epoch
         
-        requires |get_active_validator_indices(s.validators, get_current_epoch(s))| > 0
-        requires |s.validators| == |s.balances|
+    //     requires |get_active_validator_indices(s.validators, get_current_epoch(s))| > 0
+    //     requires |s.validators| == |s.balances|
         
-        ensures |get_active_validator_indices(updateProposerSlashing(s, ps).validators, get_current_epoch(s))| > 0
-    {
-        var index := ps.header_1.proposer_index; // validator to be slashed
-        var slashable_validator := s.validators[index];
-        var epoch : Epoch := get_current_epoch(s);
+    //     ensures |get_active_validator_indices(updateProposerSlashing(s, ps).validators, get_current_epoch(s))| > 0
+    // {
+    //     var index := ps.header_1.proposer_index; // validator to be slashed
+    //     var slashable_validator := s.validators[index];
+    //     var epoch : Epoch := get_current_epoch(s);
 
-        assert updateProposerSlashing(s, ps) == slash_validator(s, ps.header_1.proposer_index, get_beacon_proposer_index(s));
-        slashValidatorPreservesActivateValidators(s, ps.header_1.proposer_index, get_beacon_proposer_index(s));
-        assert |get_active_validator_indices(updateProposerSlashing(s, ps).validators, get_current_epoch(s))| > 0;
+    //     assert updateProposerSlashing(s, ps) == slash_validator(s, ps.header_1.proposer_index, get_beacon_proposer_index(s));
+    //     slashValidatorPreservesActivateValidators(s, ps.header_1.proposer_index, get_beacon_proposer_index(s));
+    //     assert |get_active_validator_indices(updateProposerSlashing(s, ps).validators, get_current_epoch(s))| > 0;
 
-    }
+    // }
 
-    lemma helperPSLemma3(s: BeaconState, ps : seq<ProposerSlashing>)
-        requires forall i :: 0 <= i < |ps| ==> ps[i].header_1.proposer_index as int < |s.validators| 
-        requires forall i :: 0 <= i < |ps| ==> !s.validators[ps[i].header_1.proposer_index].slashed 
-        requires forall i :: 0 <= i < |ps| ==> s.validators[ps[i].header_1.proposer_index].activation_epoch <= get_current_epoch(s) < s.validators[ps[i].header_1.proposer_index].withdrawable_epoch
+    // lemma helperPSLemma3(s: BeaconState, ps : seq<ProposerSlashing>)
+    //     requires forall i :: 0 <= i < |ps| ==> ps[i].header_1.proposer_index as int < |s.validators| 
+    //     requires forall i :: 0 <= i < |ps| ==> !s.validators[ps[i].header_1.proposer_index].slashed 
+    //     requires forall i :: 0 <= i < |ps| ==> s.validators[ps[i].header_1.proposer_index].activation_epoch <= get_current_epoch(s) < s.validators[ps[i].header_1.proposer_index].withdrawable_epoch
 
-        ensures forall i :: i in get_PS_validator_indices(ps) ==> 0 <= i < |s.validators|
-        ensures forall i :: i in get_PS_validator_indices(ps) ==> !s.validators[i].slashed
-        ensures forall i :: i in get_PS_validator_indices(ps) ==> s.validators[i].activation_epoch <= get_current_epoch(s) < s.validators[i].withdrawable_epoch
-    {
-        // Thanks Dafny
-    }
+    //     ensures forall i :: i in get_PS_validator_indices(ps) ==> 0 <= i < |s.validators|
+    //     ensures forall i :: i in get_PS_validator_indices(ps) ==> !s.validators[i].slashed
+    //     ensures forall i :: i in get_PS_validator_indices(ps) ==> s.validators[i].activation_epoch <= get_current_epoch(s) < s.validators[i].withdrawable_epoch
+    // {
+    //     // Thanks Dafny
+    // }
 
-    lemma helperPSLemma4(ps : seq<ProposerSlashing>)
-        requires |ps| > 0
-        requires forall i,j :: 0 <= i < j < |ps| && i != j ==> ps[i].header_1.proposer_index!= ps[j].header_1.proposer_index // ve indices are unique
-        ensures ps[|ps|-1].header_1.proposer_index as int !in get_PS_validator_indices(ps[..|ps|-1])
-    {
-        mappingPSIndices(ps[..|ps|-1]);
-        assert forall i :: 0 <= i < |ps[..|ps|-1]| ==> get_PS_validator_indices(ps[..|ps|-1])[i] == ps[i].header_1.proposer_index as int;
-    }
+    // lemma helperPSLemma4(ps : seq<ProposerSlashing>)
+    //     requires |ps| > 0
+    //     requires forall i,j :: 0 <= i < j < |ps| && i != j ==> ps[i].header_1.proposer_index!= ps[j].header_1.proposer_index // ve indices are unique
+    //     ensures ps[|ps|-1].header_1.proposer_index as int !in get_PS_validator_indices(ps[..|ps|-1])
+    // {
+    //     mappingPSIndices(ps[..|ps|-1]);
+    //     assert forall i :: 0 <= i < |ps[..|ps|-1]| ==> get_PS_validator_indices(ps[..|ps|-1])[i] == ps[i].header_1.proposer_index as int;
+    // }
 
-    lemma helperPSLemma5(s: BeaconState, ps : seq<ProposerSlashing>)
-        requires |ps| > 0
-        requires forall i,j :: 0 <= i < j < |ps| && i != j ==> ps[i].header_1.proposer_index!= ps[j].header_1.proposer_index // ve indices are unique
-        requires forall i :: 0 <= i < |ps| ==> ps[i].header_1.slot == ps[i].header_2.slot
-        requires forall i :: 0 <= i < |ps| ==> ps[i].header_1.proposer_index == ps[i].header_2.proposer_index 
-        requires forall i :: 0 <= i < |ps| ==> ps[i].header_1 == ps[i].header_2
-        requires forall i :: 0 <= i < |ps| ==> ps[i].header_1.proposer_index as int < |s.validators| 
-        requires forall i :: 0 <= i < |ps| ==> !s.validators[ps[i].header_1.proposer_index].slashed 
-        requires forall i :: 0 <= i < |ps| ==> s.validators[ps[i].header_1.proposer_index].activation_epoch <= get_current_epoch(s) < s.validators[ps[i].header_1.proposer_index].withdrawable_epoch
+    // lemma helperPSLemma5(s: BeaconState, ps : seq<ProposerSlashing>)
+    //     requires |ps| > 0
+    //     requires forall i,j :: 0 <= i < j < |ps| && i != j ==> ps[i].header_1.proposer_index!= ps[j].header_1.proposer_index // ve indices are unique
+    //     requires forall i :: 0 <= i < |ps| ==> ps[i].header_1.slot == ps[i].header_2.slot
+    //     requires forall i :: 0 <= i < |ps| ==> ps[i].header_1.proposer_index == ps[i].header_2.proposer_index 
+    //     requires forall i :: 0 <= i < |ps| ==> ps[i].header_1 == ps[i].header_2
+    //     requires forall i :: 0 <= i < |ps| ==> ps[i].header_1.proposer_index as int < |s.validators| 
+    //     requires forall i :: 0 <= i < |ps| ==> !s.validators[ps[i].header_1.proposer_index].slashed 
+    //     requires forall i :: 0 <= i < |ps| ==> s.validators[ps[i].header_1.proposer_index].activation_epoch <= get_current_epoch(s) < s.validators[ps[i].header_1.proposer_index].withdrawable_epoch
 
-        ensures forall i,j :: 0 <= i < j < |ps[..|ps|-1]| && i != j ==> ps[i].header_1.proposer_index!= ps[j].header_1.proposer_index
-        ensures forall i :: 0 <= i < |ps[..|ps|-1]| ==> ps[i].header_1.slot == ps[i].header_2.slot;
-        ensures forall i :: 0 <= i < |ps[..|ps|-1]| ==> ps[i].header_1.proposer_index == ps[i].header_2.proposer_index ;
-        ensures forall i :: 0 <= i < |ps[..|ps|-1]| ==> ps[i].header_1 == ps[i].header_2;
-        ensures forall i :: 0 <= i < |ps[..|ps|-1]| ==> ps[i].header_1.proposer_index as int < |s.validators| ;
-        ensures forall i :: 0 <= i < |ps[..|ps|-1]| ==> !s.validators[ps[i].header_1.proposer_index].slashed ;
-        ensures forall i :: 0 <= i < |ps[..|ps|-1]| ==> s.validators[ps[i].header_1.proposer_index].activation_epoch <= get_current_epoch(s) < s.validators[ps[i].header_1.proposer_index].withdrawable_epoch;
+    //     ensures forall i,j :: 0 <= i < j < |ps[..|ps|-1]| && i != j ==> ps[i].header_1.proposer_index!= ps[j].header_1.proposer_index
+    //     ensures forall i :: 0 <= i < |ps[..|ps|-1]| ==> ps[i].header_1.slot == ps[i].header_2.slot;
+    //     ensures forall i :: 0 <= i < |ps[..|ps|-1]| ==> ps[i].header_1.proposer_index == ps[i].header_2.proposer_index ;
+    //     ensures forall i :: 0 <= i < |ps[..|ps|-1]| ==> ps[i].header_1 == ps[i].header_2;
+    //     ensures forall i :: 0 <= i < |ps[..|ps|-1]| ==> ps[i].header_1.proposer_index as int < |s.validators| ;
+    //     ensures forall i :: 0 <= i < |ps[..|ps|-1]| ==> !s.validators[ps[i].header_1.proposer_index].slashed ;
+    //     ensures forall i :: 0 <= i < |ps[..|ps|-1]| ==> s.validators[ps[i].header_1.proposer_index].activation_epoch <= get_current_epoch(s) < s.validators[ps[i].header_1.proposer_index].withdrawable_epoch;
            
-    {
-    }
+    // {
+    // }
 
-    lemma helperPSLemma6(ps : seq<ProposerSlashing>)
-        requires |ps| > 0
-        ensures get_PS_validator_indices(ps[..|ps|-1]) + [ps[|ps|-1].header_1.proposer_index as int] == get_PS_validator_indices(ps)
-        ensures forall i : int :: i !in get_PS_validator_indices(ps[..|ps|-1]) && i != ps[|ps|-1].header_1.proposer_index as int ==>
-                i !in get_PS_validator_indices(ps)
-    {
-        mappingPSIndices(ps);
-        subsetMappingPSIndices(ps, |ps|-1);
-    }
+    // lemma helperPSLemma6(ps : seq<ProposerSlashing>)
+    //     requires |ps| > 0
+    //     ensures get_PS_validator_indices(ps[..|ps|-1]) + [ps[|ps|-1].header_1.proposer_index as int] == get_PS_validator_indices(ps)
+    //     ensures forall i : int :: i !in get_PS_validator_indices(ps[..|ps|-1]) && i != ps[|ps|-1].header_1.proposer_index as int ==>
+    //             i !in get_PS_validator_indices(ps)
+    // {
+    //     mappingPSIndices(ps);
+    //     subsetMappingPSIndices(ps, |ps|-1);
+    // }
 
 
     ///////////////
 
-    lemma AttestationHelperLemma(s: BeaconState, s1: BeaconState, a: Attestation)
-        requires attestationIsWellFormed(s, a);
-        requires s1.validators == s.validators
-        requires s1.slot == s.slot
-        requires s1.current_justified_checkpoint == s.current_justified_checkpoint
-        requires s1.previous_justified_checkpoint == s.previous_justified_checkpoint
-        ensures attestationIsWellFormed(s1, a);
-    { // Thanks Dafny
-    }
+    
 
     //////////////////
 
-    lemma VolExitLemma1(s: BeaconState, voluntary_exit: VoluntaryExit)
-        requires |s.validators| == |s.balances|
-        requires voluntary_exit.validator_index as int < |s.validators| 
-        requires minimumActiveValidators(s)
+    // lemma VolExitLemma1(s: BeaconState, voluntary_exit: VoluntaryExit)
+    //     requires |s.validators| == |s.balances|
+    //     requires voluntary_exit.validator_index as int < |s.validators| 
+    //     requires minimumActiveValidators(s)
         
-        requires !s.validators[voluntary_exit.validator_index].slashed
-        requires s.validators[voluntary_exit.validator_index].activation_epoch <= get_current_epoch(s) < s.validators[voluntary_exit.validator_index].withdrawable_epoch
+    //     requires !s.validators[voluntary_exit.validator_index].slashed
+    //     requires s.validators[voluntary_exit.validator_index].activation_epoch <= get_current_epoch(s) < s.validators[voluntary_exit.validator_index].withdrawable_epoch
 
-        requires s.validators[voluntary_exit.validator_index].exitEpoch == FAR_FUTURE_EPOCH
-        requires get_current_epoch(s) >= voluntary_exit.epoch
-        requires get_current_epoch(s) >= s.validators[voluntary_exit.validator_index].activation_epoch + SHARD_COMMITTEE_PERIOD 
+    //     requires s.validators[voluntary_exit.validator_index].exitEpoch == FAR_FUTURE_EPOCH
+    //     requires get_current_epoch(s) >= voluntary_exit.epoch
+    //     requires get_current_epoch(s) >= s.validators[voluntary_exit.validator_index].activation_epoch + SHARD_COMMITTEE_PERIOD 
 
-        ensures minimumActiveValidators(updateVoluntaryExit(s, voluntary_exit))
-    {
-        // var s1 := updateVoluntaryExit(s, voluntary_exit);
-        // assert get_current_epoch(s) == get_current_epoch(s1);
-        // assert exists v :: 0 <= v < |s.validators| && s.validators[v].activation_epoch <= get_current_epoch(s) < s.validators[v].exitEpoch;
-        // assert forall v :: 0 <= v < |s.validators| ==> s.validators[v].activation_epoch <= get_current_epoch(s) < s.validators[v].exitEpoch
-        //                                             ==> s1.validators[v].activation_epoch <= get_current_epoch(s1) < s1.validators[v].exitEpoch;
-        // assert exists v :: 0 <= v < |s1.validators| && s1.validators[v].activation_epoch <= get_current_epoch(s1) < s1.validators[v].exitEpoch;
-        // assert exists v :: 0 <= v < |s1.validators| && is_active_validator(s1.validators[v], get_current_epoch(s1));
-        // assert |get_active_validator_indices(s1.validators, get_current_epoch(s1))| > 0 ==> 
-        //     (exists v :: 0 <= v < |s1.validators| && is_active_validator(s1.validators[v], get_current_epoch(s1)));
-        // assert  minimumActiveValidators(s1);
-    }
+    //     ensures minimumActiveValidators(updateVoluntaryExit(s, voluntary_exit))
+    // {
+    //     // var s1 := updateVoluntaryExit(s, voluntary_exit);
+    //     // assert get_current_epoch(s) == get_current_epoch(s1);
+    //     // assert exists v :: 0 <= v < |s.validators| && s.validators[v].activation_epoch <= get_current_epoch(s) < s.validators[v].exitEpoch;
+    //     // assert forall v :: 0 <= v < |s.validators| ==> s.validators[v].activation_epoch <= get_current_epoch(s) < s.validators[v].exitEpoch
+    //     //                                             ==> s1.validators[v].activation_epoch <= get_current_epoch(s1) < s1.validators[v].exitEpoch;
+    //     // assert exists v :: 0 <= v < |s1.validators| && s1.validators[v].activation_epoch <= get_current_epoch(s1) < s1.validators[v].exitEpoch;
+    //     // assert exists v :: 0 <= v < |s1.validators| && is_active_validator(s1.validators[v], get_current_epoch(s1));
+    //     // assert |get_active_validator_indices(s1.validators, get_current_epoch(s1))| > 0 ==> 
+    //     //     (exists v :: 0 <= v < |s1.validators| && is_active_validator(s1.validators[v], get_current_epoch(s1)));
+    //     // assert  minimumActiveValidators(s1);
+    // }
 
 
     lemma helperVoluntaryExitLemma3(s: BeaconState, ve: seq<VoluntaryExit>)
@@ -330,24 +428,24 @@ module ProcessOperationsProofs {
         
     }
 
-    lemma helperVoluntaryExitLemma(s: BeaconState, exit: VoluntaryExit)
-        requires |s.validators| == |s.balances|
-        requires exit.validator_index as int < |s.validators| 
-        // requires is_active_validator(s.validators[voluntary_exit.validator_index], get_current_epoch(s))
-        // (!v.slashed) && (v.activation_epoch <= epoch < v.withdrawable_epoch)
-        requires !s.validators[exit.validator_index].slashed
-        requires s.validators[exit.validator_index].activation_epoch <= get_current_epoch(s) < s.validators[exit.validator_index].withdrawable_epoch
+    // lemma helperVoluntaryExitLemma(s: BeaconState, exit: VoluntaryExit)
+    //     requires |s.validators| == |s.balances|
+    //     requires exit.validator_index as int < |s.validators| 
+    //     // requires is_active_validator(s.validators[voluntary_exit.validator_index], get_current_epoch(s))
+    //     // (!v.slashed) && (v.activation_epoch <= epoch < v.withdrawable_epoch)
+    //     requires !s.validators[exit.validator_index].slashed
+    //     requires s.validators[exit.validator_index].activation_epoch <= get_current_epoch(s) < s.validators[exit.validator_index].withdrawable_epoch
 
-        requires s.validators[exit.validator_index].exitEpoch == FAR_FUTURE_EPOCH
-        requires get_current_epoch(s) >= exit.epoch
-        requires get_current_epoch(s) >= s.validators[exit.validator_index].activation_epoch + SHARD_COMMITTEE_PERIOD 
+    //     requires s.validators[exit.validator_index].exitEpoch == FAR_FUTURE_EPOCH
+    //     requires get_current_epoch(s) >= exit.epoch
+    //     requires get_current_epoch(s) >= s.validators[exit.validator_index].activation_epoch + SHARD_COMMITTEE_PERIOD 
         
-        ensures forall i :: 0 <= i < |s.validators| && i != exit.validator_index as int ==> updateVoluntaryExit(s, exit).validators[i].exitEpoch == s.validators[i].exitEpoch
-        ensures forall i :: 0 <= i < |s.validators| && i != exit.validator_index as int ==> updateVoluntaryExit(s, exit).validators[i].slashed == s.validators[i].slashed
-        ensures forall i :: 0 <= i < |s.validators| && i != exit.validator_index as int ==> updateVoluntaryExit(s, exit).validators[i].withdrawable_epoch == s.validators[i].withdrawable_epoch
-    {
-        // Thanks Dafny
-    }
+    //     ensures forall i :: 0 <= i < |s.validators| && i != exit.validator_index as int ==> updateVoluntaryExit(s, exit).validators[i].exitEpoch == s.validators[i].exitEpoch
+    //     ensures forall i :: 0 <= i < |s.validators| && i != exit.validator_index as int ==> updateVoluntaryExit(s, exit).validators[i].slashed == s.validators[i].slashed
+    //     ensures forall i :: 0 <= i < |s.validators| && i != exit.validator_index as int ==> updateVoluntaryExit(s, exit).validators[i].withdrawable_epoch == s.validators[i].withdrawable_epoch
+    // {
+    //     // Thanks Dafny
+    // }
 
     lemma mappingVolExitIndices(ve: seq<VoluntaryExit>)
         ensures forall i :: 0 <= i < |ve| ==> get_VolExit_validator_indices(ve)[i] == ve[i].validator_index as int
@@ -371,15 +469,15 @@ module ProcessOperationsProofs {
         }
     }
 
-    //lemma PSpreconditionLemma()
-    lemma helperVolExitLemma4(ve : seq<VoluntaryExit>)
-        requires |ve| > 0
-        requires forall i,j :: 0 <= i < j < |ve| && i != j ==> ve[i].validator_index!= ve[j].validator_index // ve indices are unique
-        ensures ve[|ve|-1].validator_index as int !in get_VolExit_validator_indices(ve[..|ve|-1])
-    {
-        mappingVolExitIndices(ve[..|ve|-1]);
-        assert forall i :: 0 <= i < |ve[..|ve|-1]| ==> get_VolExit_validator_indices(ve[..|ve|-1])[i] == ve[i].validator_index as int;
-    }
+    // //lemma PSpreconditionLemma()
+    // lemma helperVolExitLemma4(ve : seq<VoluntaryExit>)
+    //     requires |ve| > 0
+    //     requires forall i,j :: 0 <= i < j < |ve| && i != j ==> ve[i].validator_index!= ve[j].validator_index // ve indices are unique
+    //     ensures ve[|ve|-1].validator_index as int !in get_VolExit_validator_indices(ve[..|ve|-1])
+    // {
+    //     mappingVolExitIndices(ve[..|ve|-1]);
+    //     assert forall i :: 0 <= i < |ve[..|ve|-1]| ==> get_VolExit_validator_indices(ve[..|ve|-1])[i] == ve[i].validator_index as int;
+    // }
 
     
 
